Add checks for leaf package in external path -> path conversion

fstar/new/MLS.TreeSync.ExternalPath.fst
@@ -5,28 +5,58 @@ open MLS.Tree
 open MLS.Crypto
 open MLS.TreeSync.Types
 open MLS.TreeSync.ParentHash
+open MLS.TreeSync.IntegrityCheck
+open MLS.TreeSync.Extensions
+open MLS.NetworkTypes
+open MLS.NetworkBinder
+open MLS.Parser
 open MLS.Result
 
 //TODO: this function has bad complexity (because some subtrees are converted a lot of time)
 //Do we care?
-val external_pathsync_to_pathsync_aux: #l:nat -> #n:tree_size l -> #i:leaf_index n -> cs:ciphersuite -> bytes -> nat -> treesync l n -> external_pathsync l n i -> result (pathsync l n i)
-let rec external_pathsync_to_pathsync_aux #l #n #i cs parent_parent_hash nb_left_leaves t p =
+val external_pathsync_to_pathsync_aux: #l:nat -> #n:tree_size l -> #i:leaf_index n -> cs:ciphersuite -> option (sign_private_key cs & randomness (sign_nonce_length cs)) -> bytes -> nat -> treesync l n -> external_pathsync l n i -> result (pathsync l n i)
+let rec external_pathsync_to_pathsync_aux #l #n #i cs opt_sign_key parent_parent_hash nb_left_leaves t p =
   match t, p with
   | _, PLeaf lp ->
-    //TODO check that the parent hash in lp is correct
-    return (PLeaf (Some lp))
+    leaf_errors <-- check_leaf cs 0 (Some lp); //TODO hack: we know that the leaf index is only used for the errors, so we can set it to 0
+    lp <-- (
+      match opt_sign_key with
+      | None -> return lp
+      | Some (sign_key, entropy) -> (
+        if not (Seq.length parent_parent_hash < 256) then
+          internal_failure "external_pathsync_to_pathsync_aux: parent hash too long"
+        else (
+          new_extensions <-- set_parent_hash_extension lp.lp_extensions ({phen_parent_hash = parent_parent_hash});
+          let lp = ({lp with lp_extensions = new_extensions}) in
+          key_package <-- treesync_to_keypackage cs lp;
+          let leaf_package_bytes = ps_key_package_tbs.serialize (key_package_get_tbs key_package) in
+          new_signature <-- sign_sign cs sign_key leaf_package_bytes entropy;
+          return ({lp with lp_signature = new_signature})
+        )
+      )
+    );
+    let parent_hash_ext = get_parent_hash_extension lp.lp_extensions in
+    //TODO: hack while openmls' test vectors are broken
+    if not (IE_Good? leaf_errors || (match leaf_errors with |IE_Errors [IE_LeafError LIE_ExtensionsNotInCapabilities _] -> true | _ -> false)) then
+      error "external_pathsync_to_pathsync_aux: invalid leaf"
+    else if not (Some? parent_hash_ext) then
+      error "external_pathsync_to_pathsync_aux: leaf don't contain any parent hash"
+    else if not ((Some?.v parent_hash_ext).phen_parent_hash = parent_parent_hash) then
+      error "external_pathsync_to_pathsync_aux: leaf contain an invalid parent hash"
+    else
+      return (PLeaf (Some lp))
   | TSkip _ t', PSkip _ p' ->
-    result <-- external_pathsync_to_pathsync_aux cs parent_parent_hash nb_left_leaves t' p';
+    result <-- external_pathsync_to_pathsync_aux cs opt_sign_key parent_parent_hash nb_left_leaves t' p';
     return (PSkip _ result)
   | TNode _ left right, PNode np p_next ->
     let (|dir, next_i|) = child_index l i in
     let (child, sibling) = order_subtrees dir (left, right) in
     let child_nb_left_leaves = if dir = Left then nb_left_leaves else nb_left_leaves + (pow2 (l-1)) in
     parent_hash <-- compute_parent_hash_from_dir cs np.np_content parent_parent_hash nb_left_leaves t dir;
-    result_p_next <-- external_pathsync_to_pathsync_aux cs parent_hash child_nb_left_leaves child p_next;
+    result_p_next <-- external_pathsync_to_pathsync_aux cs opt_sign_key parent_hash child_nb_left_leaves child p_next;
     return (PNode (Some ({np with np_parent_hash = parent_parent_hash;})) result_p_next)
 
-val external_pathsync_to_pathsync: #l:nat -> #n:tree_size l -> #i:leaf_index n -> cs:ciphersuite -> treesync l n -> external_pathsync l n i -> result (pathsync l n i)
-let external_pathsync_to_pathsync #l #n #i cs t p =
-  external_pathsync_to_pathsync_aux cs bytes_empty 0 t p
+val external_pathsync_to_pathsync: #l:nat -> #n:tree_size l -> #i:leaf_index n -> cs:ciphersuite -> option (sign_private_key cs & randomness (sign_nonce_length cs)) -> treesync l n -> external_pathsync l n i -> result (pathsync l n i)
+let external_pathsync_to_pathsync #l #n #i cs opt_sign_key t p =
+  external_pathsync_to_pathsync_aux cs opt_sign_key bytes_empty 0 t p
 
